src/proof/create.v
@@ -98,18 +98,18 @@ Proof.
   fold new_key in Hnew_key_not_in_phys. fold new_key in Hnew_key_not_reserved.
   iAssert (⌜ abs_state !! new_key = None ⌝%I) with "[Hphys_abs_rep]" as "%Hnew_key_not_in_abs".
   { iDestruct (big_sepM2_dom with "Hphys_abs_rep") as %Hdom_eq. iPureIntro. apply not_elem_of_dom. apply not_elem_of_dom in Hnew_key_not_in_phys. set_solver. }
-  iAssert (⌜ children !! new_key = None ⌝%I) with "[Hconsistent]" as "%Hnew_key_not_in_children".
-  { iNamed "Hconsistent". iPureIntro. apply not_elem_of_dom. apply not_elem_of_dom in Hnew_key_not_in_abs. set_solver. }
+  assert (children !! new_key = None) as Hnew_key_not_in_children.
+  { destruct Hghost_well_formed. apply not_elem_of_dom. apply not_elem_of_dom in Hnew_key_not_in_abs. set_solver. }
   iAssert (⌜ abs_state !! parent_key = Some (owned_parent) ⌝%I) with "[Hown_parent Hown_abs]" as "%Hparent_key_in_abs".
   { iDestruct (map_valid with "Hown_abs Hown_parent") as %Hlookup. iPureIntro; exact Hlookup. }
   iAssert (⌜ children !! parent_key = Some (owned_child_keys) ⌝%I) with "[Hown_child_keys Hown_children]" as "%Hparent_key_in_children".
   { iDestruct (map_valid with "Hown_children Hown_child_keys") as %Hlookup. iPureIntro; exact Hlookup. }
   assert (new_key ≠ parent_key) as Hnew_key_neq_parent_key.
   { intros Heq. congruence. }
-  iAssert (⌜ <[parent_key:=owned_child_keys ∪ {[new_key]}]> children !! new_key = None ⌝%I) with "[Hconsistent]" as "%Hnew_key_not_in_children_after_update".
-  { iNamed "Hconsistent". iPureIntro. apply not_elem_of_dom. apply not_elem_of_dom in Hnew_key_not_in_abs. set_solver. }
-  iAssert (⌜ new_key ∉ owned_child_keys ⌝ %I) as "%Hnew_key_not_in_owned_child_keys".
-  { iNamed "Hconsistent". iPureIntro.
+  assert (<[parent_key:=owned_child_keys ∪ {[new_key]}]> children !! new_key = None) as Hnew_key_not_in_children_after_update.
+  { destruct Hghost_well_formed. apply not_elem_of_dom. apply not_elem_of_dom in Hnew_key_not_in_abs. set_solver. }
+  assert (new_key ∉ owned_child_keys) as Hnew_key_not_in_owned_child_keys.
+  { destruct Hghost_well_formed.
     assert (owned_child_keys ⊆ dom abs_state) as Howned_in_abs.
     { apply Hchildren_exist with (k := parent_key). exact Hparent_key_in_children. }
     apply not_elem_of_dom in Hnew_key_not_in_abs.
@@ -141,9 +141,8 @@ Proof.
       iExists copied_ptr, created_pod, created_pure_pod.
       unfold pod_rep. iFrame "#". iFrame. iPureIntro. done.
     - done. }
-  iAssert (kubernetes_state_consistent (dom used_uid') abs_state' children' fresh_keys %I) as "#Hconsistent'".
+  assert (ghost_well_formed (dom used_uid') abs_state' children' fresh_keys ) as Hghost_well_formed'.
   {
-    iNamed "Hconsistent".
     assert (dom children' = dom children ∪ {[new_key]}) as Hdom_children_eq.
     {
       unfold children'.
@@ -161,10 +160,10 @@ Proof.
     assert (obj_has_controller_parent_of (KObject.Pod created_pure_pod) (KKey.Kind' parent_key)
       (KKey.Name' parent_key) (PureObjectMeta.UID' (extract_kobject_metadata owned_parent)))
       as Hcreated_pure_pod_has_controller_parent_of_owned_parent by done.
-    iPureIntro.
-    split_and!.
-    { unfold abs_state'. unfold children'. rewrite Hdom_children_eq. rewrite dom_insert_L. set_solver. }
-    { intros k s Hlookup.
+    destruct Hghost_well_formed.
+    apply mk.
+    - unfold abs_state'. unfold children'. rewrite Hdom_children_eq. rewrite dom_insert_L. set_solver.
+    - intros k s Hlookup.
       unfold children' in Hlookup. unfold abs_state'.
       rewrite lookup_insert_Some in Hlookup.
       destruct Hlookup as [(<- & <-) | (Hk_neq & Hlookup)]; [set_solver|].
@@ -174,31 +173,28 @@ Proof.
       assert (s ⊆ dom abs_state) as s_in_abs.
       { apply Hchildren_exist with (k := k). done. }
       set_solver.
-    }
-    { intros k s child_key Hlookup Hchild_in_s.
+    - intros k s child_key Hlookup Hchild_in_s.
       unfold children' in Hlookup.
       rewrite lookup_insert_Some in Hlookup.
       destruct Hlookup as [(<- & <-) | (Hk_neq & Hlookup)]; [set_solver|].
       rewrite lookup_insert_Some in Hlookup.
       destruct Hlookup as [(<- & <-) | (Hk_neq_parent & Hlookup)].
-      - assert (child_key ∈ owned_child_keys ∨ child_key = new_key) as Hchild_cases by set_solver.
+      + assert (child_key ∈ owned_child_keys ∨ child_key = new_key) as Hchild_cases by set_solver.
         destruct Hchild_cases as [Hchild_in_owned | ->].
-        + apply Hparents_children_same_namespace with (k := parent_key) (s := owned_child_keys); done.
-        + done.
-      - apply Hparents_children_same_namespace with (k := k) (s := s); done.
-    }
-    { intros k s child_key Hlookup Hchild_in_s.
+        * apply Hparents_children_same_namespace with (k := parent_key) (s := owned_child_keys); done.
+        * done.
+      + apply Hparents_children_same_namespace with (k := k) (s := s); done.
+    - intros k s child_key Hlookup Hchild_in_s.
       unfold children' in Hlookup.
       rewrite lookup_insert_Some in Hlookup.
       destruct Hlookup as [(<- & <-) | (Hk_neq & Hlookup)]; [set_solver|].
       rewrite lookup_insert_Some in Hlookup.
       destruct Hlookup as [(<- & <-) | (Hk_neq_parent & Hlookup)].
-      - assert (child_key ∈ owned_child_keys ∨ child_key = new_key) as Hchild_cases by set_solver.
+      + assert (child_key ∈ owned_child_keys ∨ child_key = new_key) as Hchild_cases by set_solver.
         destruct Hchild_cases as [Hchild_in_owned | ->]; [|done].
         apply Hno_self_parenting with (k := parent_key) (s := owned_child_keys); done.
-      - apply Hno_self_parenting with (k := k) (s := s); done.
-    }
-    { intros k1 s1 k2 s2 Hk1_neq_k2 Hlookup1 Hlookup2.
+      + apply Hno_self_parenting with (k := k) (s := s); done.
+    - intros k1 s1 k2 s2 Hk1_neq_k2 Hlookup1 Hlookup2.
       unfold children' in Hlookup1, Hlookup2.
       rewrite lookup_insert_Some in Hlookup1.
       rewrite lookup_insert_Some in Hlookup2.
@@ -208,8 +204,8 @@ Proof.
       rewrite lookup_insert_Some in Hlookup2.
       destruct Hlookup1 as [(<- & <-) | (Hk1_neq_parent & Hlookup1)];
       destruct Hlookup2 as [(<- & <-) | (Hk2_neq_parent & Hlookup2)].
-      - done.
-      - assert (s2 ⊆ dom abs_state) as s2_in_abs.
+      + done.
+      + assert (s2 ⊆ dom abs_state) as s2_in_abs.
         { apply Hchildren_exist with (k := k2). exact Hlookup2. }
         assert (owned_child_keys ## s2) as disj.
         { apply Hchildren_disjoint with (k1 := parent_key) (k2 := k2); [|exact Hparent_key_in_children|exact Hlookup2].
@@ -217,7 +213,7 @@ Proof.
         assert (new_key ∉ dom abs_state) as key_not_in_abs.
         { apply not_elem_of_dom. exact Hnew_key_not_in_abs. }
         clear -disj s2_in_abs key_not_in_abs. set_solver.
-      - assert (s1 ⊆ dom abs_state) as s1_in_abs.
+      + assert (s1 ⊆ dom abs_state) as s1_in_abs.
         { apply Hchildren_exist with (k := k1). exact Hlookup1. }
         assert (s1 ## owned_child_keys) as disj.
         { apply Hchildren_disjoint with (k1 := k1) (k2 := parent_key); [|exact Hlookup1|exact Hparent_key_in_children].
@@ -225,98 +221,90 @@ Proof.
         assert (new_key ∉ dom abs_state) as key_not_in_abs.
         { apply not_elem_of_dom. exact Hnew_key_not_in_abs. }
         clear -disj s1_in_abs key_not_in_abs. set_solver.
-      - apply Hchildren_disjoint with (k1 := k1) (k2 := k2); done.
-    }
-    { unfold abs_state'. rewrite dom_insert_L.
+      + apply Hchildren_disjoint with (k1 := k1) (k2 := k2); done.
+    - unfold abs_state'. rewrite dom_insert_L.
       assert (new_key ∉ fresh_keys) as Hkey_not_in_fresh.
       { intros Hin. apply Hfresh_keys_reserved in Hin. done. }
       clear -Hfresh_keys_absent Hkey_not_in_fresh.
       set_solver.
-    }
-    { apply Hfresh_keys_reserved. }
-    { intros k1 k2 obj1 obj2 Hlookup1 Hlookup2 Huid_eq.
+    - apply Hfresh_keys_reserved.
+    - intros k1 k2 obj1 obj2 Hlookup1 Hlookup2 Huid_eq.
       unfold abs_state' in Hlookup1, Hlookup2.
       rewrite lookup_insert_Some in Hlookup1.
       rewrite lookup_insert_Some in Hlookup2.
       destruct Hlookup1 as [(<- & <-) | (Hk1_neq & Hlookup1)];
       destruct Hlookup2 as [(<- & <-) | (Hk2_neq & Hlookup2)].
-      - done.
-      - assert ((extract_kobject_metadata obj2).(PureObjectMeta.UID') ∈ dom used_uid) as Hobj2_uid_in_used.
+      + done.
+      + assert ((extract_kobject_metadata obj2).(PureObjectMeta.UID') ∈ dom used_uid) as Hobj2_uid_in_used.
         { apply Hexisting_uid_is_used with (k := k2). done. }
         rewrite <-Huid_eq, Hcreated_pure_pod_uiq_eq in Hobj2_uid_in_used. done.
-      - assert ((extract_kobject_metadata obj1).(PureObjectMeta.UID') ∈ dom used_uid) as Hobj1_uid_in_used.
+      + assert ((extract_kobject_metadata obj1).(PureObjectMeta.UID') ∈ dom used_uid) as Hobj1_uid_in_used.
         { apply Hexisting_uid_is_used with (k := k1). done. }
         rewrite Huid_eq Hcreated_pure_pod_uiq_eq in Hobj1_uid_in_used. done.
-      - apply Hno_duplicate_uid with (obj1 := obj1) (obj2 := obj2); done.
-    }
-    { intros k obj Hlookup_abs_state. unfold abs_state', used_uid'.
+      + apply Hno_duplicate_uid with (obj1 := obj1) (obj2 := obj2); done.
+    - intros k obj Hlookup_abs_state. unfold abs_state', used_uid'.
       rewrite dom_insert_L. rewrite lookup_insert_Some in Hlookup_abs_state.
       destruct Hlookup_abs_state as [(<- & <-) | (Hk_neq & Hlookup_abs_state)]; [set_solver|set_solver].
-    }
-    { intros key_p obj_p key_c obj_c s Hlookup_p Hlookup_c Hlookup_children.
+    - intros key_p obj_p key_c obj_c s Hlookup_p Hlookup_c Hlookup_children.
       unfold abs_state' in Hlookup_p, Hlookup_c.
       unfold children' in Hlookup_children.
       rewrite lookup_insert_Some in Hlookup_p.
       rewrite lookup_insert_Some in Hlookup_c.
       rewrite lookup_insert_Some in Hlookup_children.
       split.
-      { intros Hkey_c_in_s.
+      + intros Hkey_c_in_s.
         destruct Hlookup_children as [(<- & <-) | (Hkey_p_neq & Hlookup_children)]; [done|].
         destruct Hlookup_p as [(<- & <-) | (Hkey_p_neq' & Hlookup_p)]; [done|].
         destruct Hlookup_c as [(<- & <-) | (Hkey_c_neq & Hlookup_c)].
-        - rewrite lookup_insert_Some in Hlookup_children.
+        * rewrite lookup_insert_Some in Hlookup_children.
           destruct Hlookup_children as [(<- & <-) | (Hkey_p_neq'' & Hlookup_children)].
-          + rewrite Hparent_key_in_abs in Hlookup_p. injection Hlookup_p as <-. done.
-          + eapply Hchildren_exist in Hlookup_children. apply not_elem_of_dom in Hnew_key_not_in_abs. set_solver.
-        - rewrite lookup_insert_Some in Hlookup_children.
+          -- rewrite Hparent_key_in_abs in Hlookup_p. injection Hlookup_p as <-. done.
+          -- eapply Hchildren_exist in Hlookup_children. apply not_elem_of_dom in Hnew_key_not_in_abs. set_solver.
+        * rewrite lookup_insert_Some in Hlookup_children.
           destruct Hlookup_children as [(<- & <-) | (Hkey_p_neq'' & Hlookup_children)].
-          + eapply Hchildren_point_to_parent; [done|done|done|]. set_solver.
-          + eapply Hchildren_point_to_parent; [done|done|done|done].
-      }
-      { intros Hobj_has_controller_parent_of.
+          -- eapply Hchildren_point_to_parent; [done|done|done|]. set_solver.
+          -- eapply Hchildren_point_to_parent; [done|done|done|done].
+      + intros Hobj_has_controller_parent_of.
         destruct Hlookup_c as [(<- & <-) | (Hkey_c_neq & Hlookup_c)].
-        - assert (well_formed_kobject (KObject.Pod created_pure_pod)) as Hwell_formed_kobject by done.
+        * assert (well_formed_kobject (KObject.Pod created_pure_pod)) as Hwell_formed_kobject by done.
           pose proof (well_formed_obj_has_at_most_one_controller_parent (KObject.Pod created_pure_pod) Hwell_formed_kobject
             _ _ _ _ _ _ Hobj_has_controller_parent_of Hcreated_pure_pod_has_controller_parent_of_owned_parent) as (Hkind_eq & Hname_eq & Huid_eq).
           destruct Hlookup_p as [(<- & <-) | (Hkey_p_neq & Hlookup_p)].
-          + exfalso.
+          -- exfalso.
             pose proof (Hexisting_uid_is_used parent_key owned_parent Hparent_key_in_abs).
             rewrite Hcreated_pure_pod_uiq_eq in Huid_eq.
             rewrite <-Huid_eq in H. done.
-          + pose proof (Hno_duplicate_uid _ _ _ _ Hlookup_p Hparent_key_in_abs Huid_eq) as ->.
+          -- pose proof (Hno_duplicate_uid _ _ _ _ Hlookup_p Hparent_key_in_abs Huid_eq) as ->.
             destruct Hlookup_children as [(Hkey_p_eq_new & <-) | (Hkey_p_neq' & Hlookup_children)]; [done|].
             rewrite lookup_insert_Some in Hlookup_children.
             destruct Hlookup_children as [(Hkey_p_eq_new & <-) | (Hkey_p_neq'' & Hlookup_children)]; [set_solver|done].
-        - destruct Hlookup_p as [(<- & <-) | (Hkey_p_neq & Hlookup_p)].
-          + rewrite Hcreated_pure_pod_uiq_eq in Hobj_has_controller_parent_of.
+        * destruct Hlookup_p as [(<- & <-) | (Hkey_p_neq & Hlookup_p)].
+          -- rewrite Hcreated_pure_pod_uiq_eq in Hobj_has_controller_parent_of.
             pose proof (Hparent_uid_is_used _ _ _ _ _ Hlookup_c Hobj_has_controller_parent_of).
             done.
-          + destruct Hlookup_children as [(Hkey_p_eq_new & <-) | (Hkey_p_neq' & Hlookup_children)]; [done|].
+          -- destruct Hlookup_children as [(Hkey_p_eq_new & <-) | (Hkey_p_neq' & Hlookup_children)]; [done|].
             rewrite lookup_insert_Some in Hlookup_children.
             destruct Hlookup_children as [(<- & <-) | (Hkey_p_neq'' & Hlookup_children)].
-            * rewrite Hparent_key_in_abs in Hlookup_p. injection Hlookup_p as <-.
+            ++ rewrite Hparent_key_in_abs in Hlookup_p. injection Hlookup_p as <-.
               pose proof ((proj2 (Hchildren_point_to_parent _ _ _ _ _ Hparent_key_in_abs Hlookup_c Hparent_key_in_children))).
               set_solver.
-            * pose proof ((proj2 (Hchildren_point_to_parent _ _ _ _ _ Hlookup_p Hlookup_c Hlookup_children)) Hobj_has_controller_parent_of).
+            ++ pose proof ((proj2 (Hchildren_point_to_parent _ _ _ _ _ Hlookup_p Hlookup_c Hlookup_children)) Hobj_has_controller_parent_of).
               done.
-      }
-    }
-    { intros k obj kind name uid Hlookup_abs Hhas_parent.
+    - intros k obj kind name uid Hlookup_abs Hhas_parent.
       unfold abs_state' in Hlookup_abs.
       rewrite lookup_insert_Some in Hlookup_abs.
       destruct Hlookup_abs as [(<- & <-) | (Hk_neq & Hlookup_abs)].
-      - assert (well_formed_kobject (KObject.Pod created_pure_pod)) as Hwell_formed_kobject by done.
+      + assert (well_formed_kobject (KObject.Pod created_pure_pod)) as Hwell_formed_kobject by done.
         pose proof (well_formed_obj_has_at_most_one_controller_parent (KObject.Pod created_pure_pod) Hwell_formed_kobject
           _ _ _ _ _ _ Hhas_parent Hcreated_pure_pod_has_controller_parent_of_owned_parent) as (Hkind_eq & Hname_eq & ->).
         pose proof (Hexisting_uid_is_used parent_key owned_parent Hparent_key_in_abs).
         unfold used_uid'. set_solver.
-      - pose proof (Hparent_uid_is_used k obj kind name uid Hlookup_abs Hhas_parent).
+      + pose proof (Hparent_uid_is_used k obj kind name uid Hlookup_abs Hhas_parent).
         unfold used_uid'. set_solver.
-    }
   }
   wp_apply (wp_Mutex__Unlock _ (is_kubernetes_state_inner γ_state γ_children γ_fresh_keys)
     with "[$Hown_Mutex $Hstate_m_addr $Hstate_used_uid_addr $Hstate_rvc_addr $Hown_phys $Hown_used_uid $Hown_abs $Hphys_abs_rep $Hown_children $Hown_fresh_keys]").
-  { iFrame "#". }
+  { iFrame "#". done. }
   iApply "HΦ". iFrame "Hreturned_ptr". iFrame. done.
 Qed.
 
